\lecture{13}{Nov 4 2024 Mon (13:02:06)}{Properties of Infinite Series}

\section{Properties of Infinite Series}
\label{sec:properties_of_infinite_series}

Just as we had an algebraic limit theorem for sequences, we have a similar
theorem for series.
\begin{theorem}[Algebraic Limit Theorem for Series] If $\sum_{k=1}^{\infty} a_k
  = A$ and $\sum_{k=1}^{\infty} b_k = B$, then
  \begin{enumerate}
    \item $\sum_{k=1}^{\infty} ca_k = cA$ for all $c \in \R$.
    \item $\sum_{k=1}^{\infty} (a_k + b_k) = A + B$.
  \end{enumerate}
\end{theorem}

\begin{proof}\leavevmode
  \begin{enumerate}
    \item Let $S_n = \sum_{k=1}^n a_k$. Then, $\lim_{m \to \infty} S_m = A$.
      Thus, by the Algebraic Limit Theorem for Sequences, $c\lim_{m \to \infty}
      S_m = \lim_{m \to \infty} (cS_m) = cA$. Thus, $\sum_{k=1}^{\infty} ca_k =
      cA$.

    \item Let $S_n = \sum_{k=1}^n a_k$ and $T_n = \sum_{k=1}^n b_k$. Then,
      $\lim_{m \to \infty} S_m = A$ and $\lim_{m \to \infty} T_m = B$. Thus, by
      the Algebraic Limit Theorem for Sequences, $\lim_{m \to \infty} (S_m +
      T_m) = A + B$. Thus, $\sum_{k=1}^{\infty} (a_k + b_k) = A + B$. \qedhere
  \end{enumerate}
\end{proof}

Just as we had the Cauchy criterion for sequences, we have a similar criterion
for series.
\begin{theorem}[Cauchy Criterion for Series]
  The series $\sum_{k=1}^{\infty} a_k$ converges if and only if, given $\epsilon
  > 0$, there exists an $N \in \N$ such that whenever $n > m > N$, it follows
  that
  \[%
    \lvert a_{m+1} + a_{m+2} + \cdots + a_n \rvert < \epsilon
  .\]%
\end{theorem}

\begin{proof}
  Notice that
  \[%
    \left\lvert \sum_{k=1}^n a_k - \sum_{k=1}^m a_k \right\rvert = \lvert S_n - S_m \rvert = \lvert a_{m+1} + a_{m+2} + \cdots + a_n \rvert
  .\]%
  Thus, the series converges if and only if the sequence of partial sums is a
  Cauchy sequence.
\end{proof}

This is a very powerful criterion. We use this theorem to prove all of the basic
tests for series in section \ref{sub_sec:conversion_tests}.

\begin{definition}[Absolute Convergence]
  A series $\sum_{k=1}^{\infty} a_k$ is said to \textit{converge absolutely} if
  the series $\sum_{k=1}^{\infty} \lvert a_k \rvert$ converges.
\end{definition}

\begin{definition}[Conditional Convergence]
  A series $\sum_{k=1}^{\infty} a_k$ is said to \textit{converge conditionally}
  if the series $\sum_{k=1}^{\infty} a_k$ converges, but the series
  $\sum_{k=1}^{\infty} \lvert a_k \rvert$ diverges.
\end{definition}

\subsection{Conversion Tests}
\label{sub_sec:conversion_tests}

Now, we can start proving tests that have some substance.

\begin{lemma}
  If the series $\sum_{k=1}^{\infty} a_k$ converges, then $a_k \to 0$.
\end{lemma}

\begin{proof}
  Let $S_n = \sum_{k=1}^n a_k$. Then, $a_n = S_n - S_{n-1}$. Since the series
  converges, the sequence of partial sums is Cauchy. Thus, given $\epsilon > 0$,
  there exists an $N \in \N$ such that whenever $n > m > N$, it follows that
  \[%
    \lvert S_n - S_m \rvert = \lvert a_{m+1} + a_{m+2} + \cdots + a_n \rvert < \epsilon
  .\]%
  In particular, if we take $m = n - 1$, we have
  \[%
    \lvert a_n \rvert = \lvert S_n - S_{n-1} \rvert < \epsilon
  .\]%
  Thus, $a_n \to 0$.
\end{proof}

\begin{note}
  The converse isn't true. Take, for example, the harmonic series
  $\sum_{k=1}^{\infty} \frac{1}{k}$. This series diverges, but $\frac{1}{k} \to
  0$.
\end{note}

\begin{lemma}[Absolute Convergence Test]
  If $\sum_{k=1}^{\infty} \lvert a_k \rvert$ converges, then
  $\sum_{k=1}^{\infty} a_k$ converges.
\end{lemma}

\begin{proof}
  Assume $\sum_{k=1}^{\infty} \lvert a_k \rvert$ converges. Let $\epsilon > 0$.
  Then, there exists an $N \in \N$ such that for every $n > m > N$, we have
  \[%
    \lvert a_{m+1} \rvert + \lvert a_{m+2} \rvert + \cdots + \lvert a_n \rvert < \epsilon
  .\]%
  Notice that
  \[%
    \lvert a_{m+1} + a_{m+2} + \cdots + a_n \rvert \leq \lvert a_{m+1} \rvert + \lvert a_{m+2} \rvert + \cdots + \lvert a_n \rvert < \epsilon
  .\]%
  Thus, by the Cauchy Criterion for Series, $\sum_{k=1}^{\infty} a_k$ converges.
\end{proof}

\begin{lemma}[Comparison Test]
  Assume $(a_k)$ and $(b_k)$ are sequences satisfying $(\forall k \in \N)[0 \le a_k \le b_k]$
  \begin{enumerate}
    \item If $\sum_{k=1}^{\infty} b_k$ converges, then $\sum_{k=1}^{\infty} a_k$ converges.

    \item If $\sum_{k=1}^{\infty} a_k$ diverges, then $\sum_{k=1}^{\infty} b_k$ diverges.
  \end{enumerate}
\end{lemma}

\begin{proof}\leavevmode
  Both statements follow directly from the Cauchy Criterion for Series.
  \[%
    \lvert a_{m+1} + a_{m+2} + \cdots + a_n \rvert \le \lvert b_{m+1} + b_{m+2} + \cdots + b_n \rvert
  .\]%
  If the right-hand side is less than $\epsilon$, then the left-hand side is
  less than $\epsilon$. Thus, the series converges. The second statement follows
  from the contrapositive of the first statement.
\end{proof}

\begin{lemma}[Limit Comparison Test]
  Assume $(a_k)$ and $(b_k)$ are sequences satisfying $(\forall k \in \N)[0 < a_k \le b_k]$. If
  \[%
    \lim_{k \to \infty} \frac{a_k}{b_k} = c
  ,\]%
  where $c$ is a positive real number, then $\sum_{k=1}^{\infty} a_k$ converges
  if and only if $\sum_{k=1}^{\infty} b_k$ converges.
\end{lemma}

\begin{proof}
  Let $c > 0$ such that $\lim_{k \to \infty} \frac{a_k}{b_k} = c$. This means
  for any $\epsilon > 0$, there exists an $N \in \N$ such that for all $k \geq
  N$, we have
  \[%
    c - \epsilon < \frac{a_k}{b_k} < c + \epsilon
  .\]%
  Multiplying through by $b_k$ (which is positive), we get
  \[%
    (c - \epsilon)b_k < a_k < (c + \epsilon)b_k
  .\]%
  Choose $\epsilon$ such that $0 < \epsilon < c$, so $c - \epsilon > 0$. For $k
  \geq N$, we now have
  \[%
    0 < (c - \epsilon) b_k \leq a_k \leq (c + \epsilon) b_k
  .\]%

  \begin{enumerate}
    \item Convergence of $\sum_{k=1}^{\infty} b_k$:

      If $\sum_{k=1}^{\infty} b_k$ converges, then $(c -
      \epsilon)\sum_{k=1}^{\infty} b_k$ converges because $c - \epsilon > 0$ is
      a constant multiple. By the Comparison Test applied to $(c - \epsilon)b_k
      \leq a_k$, it follows that $\sum_{k=1}^{\infty} a_k$ also converges.

    \item Case 2: Divergence of $\sum_{k=1}^{\infty} b_k$:

      If $\sum_{k=1}^{\infty} b_k$ diverges, then $(c +
      \epsilon)\sum_{k=1}^{\infty} b_k$ also diverges because $c + \epsilon > 0$
      is a constant multiple. By the Comparison Test applied to $a_k \geq (c -
      \epsilon)b_k$, it follows that $\sum_{k=1}^{\infty} a_k$ also diverges.
  \end{enumerate}

  Hence, $\sum_{k=1}^{\infty} a_k$ converges if and only if $\sum_{k=1}^{\infty}
  b_k$ converges.
\end{proof}

\begin{lemma}[Ratio Test]
  Let $(a_n)$ be a sequence. If
  \[%
    \lim_{n \to \infty} \left\lvert \frac{a_{n+1}}{a_n} \right\rvert = L
  ,\]%
  then
  \begin{enumerate}
    \item If $L < 1$, then $\sum_{n=1}^{\infty} a_n$ converges absolutely.

    \item If $L > 1$, then $\sum_{n=1}^{\infty} a_n$ diverges.

    \item If $L = 1$, then the test is inconclusive.
  \end{enumerate}
\end{lemma}

\begin{proof}\leavevmode
  Let $L = \lim_{n \to \infty} \left\lvert \frac{a_{n+1}}{a_n} \right\rvert$.
  \begin{enumerate}
    \item $L < 1$:

      Choose $\epsilon > 0$ such that $L + \epsilon < 1$. By the definition of
      the limit,
      \[%
        (\exists N \in \N)(\forall n \ge N)\left[\left\lvert \frac{a_{n+1}}{a_n} \right\rvert < L + \epsilon\right]
      .\]%
      This implies that for $n \geq N$
      \[%
        \lvert a_{n+1} \rvert < (L + \epsilon) \lvert a_n \rvert
      .\]%
      Iterating this inequality, we get
      \[%
        \lvert a_{n+1} \rvert < (L + \epsilon)^{n-N+1} \lvert a_N \rvert
      .\]%
      Since $L + \epsilon < 1$, the geometric series $\sum_{n=N}^{\infty} (L +
      \epsilon)^{n-N+1}$ converges. Therefore, by the Comparison Test,
      $\sum_{n=N}^{\infty} \lvert a_n \rvert$ converges, which implies that
      $\sum_{n=1}^{\infty} \lvert a_n \rvert$ converges. Thus,
      $\sum_{n=1}^{\infty} a_n$ converges absolutely.

    \item $L > 1$:

      Choose $\epsilon > 0$ such that $L - \epsilon > 1$. By the definition of
      the limit,
      \[%
        (\exists N \in \N)(\forall n \ge N)\left[\left\lvert \frac{a_{n+1}}{a_n} \right\rvert > L - \epsilon\right]
      .\]%
      This implies that for $n \geq N$
      \[%
        \lvert a_{n+1} \rvert > (L - \epsilon) \lvert a_n \rvert
      .\]%
      Iterating this inequality, we get
      \[%
        \lvert a_{n+1} \rvert > (L - \epsilon)^{n-N+1} \lvert a_N \rvert
      .\]%
      Since $L - \epsilon > 1$, the terms $\lvert a_n \rvert$ do not approach
      zero, and hence $\sum_{n=1}^{\infty} \lvert a_n \rvert$ diverges. Thus,
      $\sum_{n=1}^{\infty} a_n$ diverges.

    \item $L = 1$:

      The test provides no information about the convergence or divergence of
      the series. For example, the series $\sum_{n=1}^{\infty} \frac{1}{n}$
      diverges, but $\sum_{n=1}^{\infty} \frac{1}{n^2}$ converges, and both
      satisfy $\lim_{n \to \infty} \left\lvert \frac{a_{n+1}}{a_n} \right\rvert
      = 1$. Therefore, the test is inconclusive in this case. \qedhere
  \end{enumerate}
\end{proof}

\begin{lemma}[Root Test]
  Let $(a_n)$ be a sequence. If
  \[%
    \limsup_{n \to \infty} \sqrt[n]{\lvert a_n \rvert} = L
  ,\]%
  then
  \begin{enumerate}
    \item If $L < 1$, then $\sum_{n=1}^\infty a_n$ converges absolutely.
    \item If $L > 1$, then $\sum_{n=1}^\infty a_n$ diverges.
    \item If $L = 1$, then the test is inconclusive.
  \end{enumerate}
\end{lemma}

\begin{proof}
  Let $L = \limsup_{n \to \infty} \sqrt[n]{\lvert a_n \rvert}$.

  \begin{enumerate}
    \item $L < 1$:

      Choose $\epsilon > 0$ such that $L + \epsilon < 1$. By the definition of
      the $\limsup$, there exists $N \in \mathbb{N}$ such that for all $n \geq
      N$
      \[%
        \sqrt[n]{\lvert a_n \rvert} < L + \epsilon
      .\]%
      Raising both sides to the $n$th power, we have
      \[%
        (\forall n \geq N)\left[\lvert a_n \rvert < (L + \epsilon)^n\right]
      .\]%
      Since $L + \epsilon < 1$, the series $\sum_{n=N}^\infty (L + \epsilon)^n$
      converges because it is a geometric series with ratio less than $1$. By
      the Comparison Test, $\sum_{n=N}^\infty \lvert a_n \rvert$ converges, and
      therefore $\sum_{n=1}^\infty \lvert a_n \rvert$ converges. Thus,
      $\sum_{n=1}^\infty a_n$ converges absolutely.

    \item $L > 1$:

      By the definition of $\limsup$, there exists a subsequence $(a_{n_k})$
      such that
      \[%
        \sqrt[n_k]{\lvert a_{n_k} \rvert} \to L~\textrm{as}~k \to \infty
      .\]%
      Since $L > 1$, for sufficiently large $k$, we have
      \[%
        \sqrt[n_k]{\lvert a_{n_k} \rvert} > 1
      ,\]%
      which implies
      \[%
        \lvert a_{n_k} \rvert > 1^n = 1
      .\]%
      Thus, $\lvert a_{n_k} \rvert$ does not approach $0$, so the series
      $\sum_{n=1}^\infty a_n$ diverges.

    \item $L = 1$:

      The test is inconclusive because series with $L = 1$ may
      either converge or diverge. For instance
      \[%
        \sum_{n=1}^\infty \frac{1}{n^2}~\textrm{converges, while}~\sum_{n=1}^\infty \frac{1}{n}~\textrm{diverges}
      .\]%
      Both of these series satisfy $\limsup_{n \to \infty} \sqrt[n]{\lvert a_n
      \rvert} = 1$.\qedhere
  \end{enumerate}
\end{proof}

\begin{lemma}[Alternating Series Test]
  Let $(a_n)$ be a sequence satisfying the following requirements
  \begin{enumerate}
    \item $a_1 \ge a_2 \ge a_3 \ge \cdots \ge a_n \ge a_{n+1} \ge \cdots$,

    \item $a_n \to 0$,
  \end{enumerate}
  Then, the alternating series $\sum_{n=1}^{\infty} (-1)^{n+1} a_n$ converges.
\end{lemma}

\begin{proof}
  Let $S_n = \sum_{k=1}^n (-1)^{k+1} a_k$. Then, $S_{2n} = a_1 - a_2 + a_3 - a_4
  + \cdots + a_{2n-1} - a_{2n}$. Since $a_n \to 0$, we have
  \[%
    \lvert S_{2n} - S_{2n-2} \rvert = \lvert a_{2n-1} - a_{2n} \rvert \to 0
  .\]%
  Thus, $(S_{2n})$ is a Cauchy sequence. Similarly, $(S_{2n+1})$ is also a
  Cauchy sequence. Thus, both sequences converge. Since the series is the sum of
  these two sequences, the series converges.
\end{proof}

\begin{lemma}[Condensation Test]
  Suppose $(b_n)$ is decreasing and satisfies $b_n \ge 0$ for all $n \in \N$.
  Then, the series $\sum_{n=1}^{\infty} b_n$ converges if and only if the series
  \[%
    \sum_{n=0}^{\infty} 2^nb_{2^n} = b_1 + 2b_2 + 4b_4 + 8b_8 + 16b_{16} + \cdots
  ,\]%
  converges.
\end{lemma}

\begin{proof}
  First, assume that $\sum_{n=0}^{\infty} 2^nb_{2^n}$ converges. Then, the
  partial sum
  \[%
    T_k = b_1 + 2b_2 + 4b_4 + \cdots + 2^kb_{2^k}
  ,\]%
  is bounded, by some number $M$. Because $b_n \ge 0$, we know that the partial
  sums are increasing. Let $S_m = b_1 + b_2 + b_3 + \cdots + b_m$. Fix $m$ and
  let $k$ be large enough to ensure $m \le 2_{k+1} - 1$. Then, $S_m \le S_{2^k +
  1} - 1$ and
  \begin{align*}
    S_{2^{k+1}} - 1 &= b_1 + (b_2 + b_3) + (b_4 + \cdots + b_7) + \cdots + (b_{2^k} + \cdots + b_{2^{k+1} - 1}) \\
                    &\le b_1 + 2b_2 + 4b_4 + \cdots + 2^kb_{2^k} \\
                    &= T_k
  .\end{align*}
  Therefore, $S_m \le T_k \le M$ for all $m \in \N$. This implies that $(S_m)$
  is bounded and therefore converges.
\end{proof}

This is a more general statement of the statement that the sum
$\sum_{n=1}^{\infty} \frac{1}{n}$ diverges and that $\sum_{n=1}^{\infty}
\frac{1}{n^{\rho}}$ converges for $\rho > 1$.

\begin{corollary}[P-Series Test]
  The series
  \[%
    \sum_{n=1}^{\infty} \frac{1}{n^{\rho}}
  .\]%
  converges if and only if $\rho > 1$.
\end{corollary}

\begin{proof}
  Let $b_n = \frac{1}{n^{\rho}}$. By the Cauchy Condensation Test, the series
  $\sum_{n=1}^{\infty} b_n$ converges if and only if the series
  \[%
    \sum_{n=0}^{\infty} 2^n \cdot \frac{1}{(2^n)^{\rho}} = \sum_{n=0}^{\infty} \frac{1}{2^{n(\rho-1)}}
  .\]%
  converges. The latter is a geometric series with common ratio $r =
  \frac{1}{2^{\rho-1}}$. A geometric series converges if and only if $\lvert r
  \rvert < 1$. Thus, $\lvert r \rvert < 1$ implies
  \[%
    \frac{1}{2^{\rho-1}} < 1,
  \]%
  which holds if and only if $\rho - 1 > 0$, or equivalently, $\rho > 1$.
  Therefore, $\sum_{n=1}^{\infty} \frac{1}{n^{\rho}}$ converges if and only if
  $\rho > 1$.
\end{proof}

\begin{lemma}[Abel's Test]
\end{lemma}

\begin{proof}
\end{proof}

\begin{lemma}[Dirichlet's Test]
\end{lemma}

\begin{proof}
\end{proof}

% subsection conversion_tests (end)

\subsection{Rearrangements}
\label{sub_sec:rearrangements}



% subsection rearrangements (end)

\subsection{Double Summations of Infinite Series}
\label{sub_sec:double_summations_of_infinite_series}

\begin{note}
  These next two sections aren't a part of the course, but they are interesting
  to know and in future courses, professors assume you already know this, like
  in Complex Analysis.
\end{note}

\begin{definition}[Iterated Summation]
  Given a doubly indexed array of real numbers $\{a_{ij} \mid i, j \in \N\}$,
  the \textit{iterated sum} of the array is defined as
  \[%
    S_{mn} = \sum_{i=1}^m \sum_{j=1}^n a_{ij} = \sum_{i,j=1}^{\infty} a_{ij}
  .\]%
\end{definition}

\begin{note}
  Notice that the order of summation matters, giving us
  \[%
    \sum_{i=1}^{\infty} \sum_{j=1}^{\infty} a_{ij} \neq \sum_{j=1}^{\infty} \sum_{i=1}^{\infty} a_{ij}
  .\]%
  But when it comes to using partial sums, as long as the series converges, then
  the order of summation doesn't matter.
\end{note}

% subsection double_summations_of_infinite_series (end)

\subsection{Products of Infinite Series}
\label{sub_sec:products_of_infinite_series}



% subsection products_of_infinite_series (end)

% section properties_of_infinite_series (end)
